"Fp2 ring operations for reification w. proofs"

Examples/p127/Example127Montgomery.v
@@ -9,58 +9,9 @@ Require Import Crypto.Arithmetic.UniformWeight.
 Require Import Crypto.Stringification.IR.
 Require Import QuadraticFieldExtensions.
 Require Import Coqprime.elliptic.GZnZ.
-
-Import ListNotations.
-
-Definition s := (2 ^ 127)%Z.
-Definition c := [(1, 1)].
-Definition p := Eval compute in (s - Associational.eval c).
-Hypothesis p_prime: prime p.
-Hypothesis p_ge2: 2 < p.
-Hypothesis pmod: p mod 4 =? 3 = true.
-Definition w := uweight 64.
-Notation "n 'zmod' p" := (mkznz p (n mod p) (modz p n)) (at level 90).
-Check QuadraticFieldExtensions.Quad_non_res.
-Lemma quad_res_minus_1: Quad_non_res p = ((-1) zmod p).
-Proof.
-    reflexivity.
-Qed.
-
-(*
-Lemma s_nz: s <> 0.
-Proof. unfold s; auto with zarith. Qed.
-
-Lemma m_nz: s - Associational.eval c <> 0.
-Proof. unfold s, c; simpl; auto with zarith. Qed.
-
-Definition force_carry l := (Positional.chained_carries w 3 s c l [0%nat;1%nat;2%nat]).
-
-Definition m' := 1.
-Definition r := 2 ^ 64.
-
-Lemma m'_correct : (p * m') mod r = (-1) mod r.
-Proof. auto with zarith. Qed.
-*)
-
-Notation "x +Fp y" := (GZnZ.add p x y) (at level 100).
-Notation "x *Fp y" := (GZnZ.mul p x y) (at level 90).
-Notation "x -Fp y" := (GZnZ.sub p x y) (at level 100).
-
-
-Check WordByWordMontgomery.from_montgomerymod 64 2 p 4.
-
-Definition mul127 x y := (WordByWordMontgomery.mulmod 64 2 p 1 x y).
-Definition add127 x y := (WordByWordMontgomery.addmod 64 2 p x y).
-Definition sub127 x y := (WordByWordMontgomery.submod 64 2 p x y).
-Definition enc127 z := Positional.encode w 2 s c z.
-Definition tomont127 z := WordByWordMontgomery.encodemod 64 2 p 1 z.
-Definition eval127' z := (Positional.eval w 2 z).
-Definition frommont127 z := WordByWordMontgomery.from_montgomerymod 64 2 p 1 z.
-Definition eval127 z := @WordByWordMontgomery.eval 64 2 (WordByWordMontgomery.from_montgomerymod 64 2 p 1 z).
-
-
-
-(** * Push-Button Synthesis Examples *)
+Require Import Field_theory.
+Require Import Ring_theory.
+Require Import Crypto.Util.LetIn.
 Require Import Coq.Strings.String.
 Require Import Coq.ZArith.ZArith.
 Require Import Coq.Lists.List.
@@ -72,91 +23,55 @@ Require Import Crypto.Arithmetic.Core.
 Require Import Crypto.Arithmetic.ModOps.
 Require Import Crypto.Arithmetic.Primitives.
 Require Import Crypto.BoundsPipeline.
+From Coqprime Require Import LucasLehmer.
 Import ListNotations.
-Local Open Scope Z_scope. Local Open Scope list_scope.
-
-Import
-  Language.Compilers
-  Stringification.C.Compilers.
+Import Language.Compilers Stringification.C.Compilers.
 Import Compilers.API.
-
 Import Associational Positional.
+Local Open Scope Z_scope.
+Local Open Scope list_scope.
 
-Local Instance : split_mul_to_opt := None.
-Local Instance : split_multiret_to_opt := None.
-Local Instance : unfold_value_barrier_opt := true.
-Local Instance : only_signed_opt := false.
-Local Instance : no_select_size_opt := None.
-Local Existing Instance default_low_level_rewriter_method.
-(*
-Check mulmod.
-Check (weight 51 1).
-Check w.
+(*Definitions and notation*)
 
-About mulmod.
+Definition s := (2 ^ 127)%Z.
+Definition c := [(1, 1)].
+Definition p := Eval compute in (s - Associational.eval c).
+Definition w := uweight 64.
+Notation "n 'zmod' p" := (mkznz p (n mod p) (modz p n)) (at level 90).
 
-Check mulmod w s c 2.
-Check mul127.
-(*
-Time Redirect "log" Compute
-     (Pipeline.BoundsPipeline
-        true None [64; 128]
-        ltac:(let r := Reify (fun f g => mul127 f g) in
-              exact r)
-               (Some (repeat (@None _) 2), ((Some (repeat (@None _) 2), tt)))
-               ZRange.type.base.option.None).
-*)
-Check addcarryx 64.
-Check mul127.
+(*A few results on prime and base field.*)
+Lemma p_ge2: 2 < p.
+Proof. unfold p; lia. Qed.
 
-Check hd.
-Check tl.
+Lemma quad_res_minus_1: Quad_non_res p = ((-1) zmod p).
+Proof. reflexivity. Qed.
 
-About WordByWordMontgomery.mulmod.
-Definition mp := 10540996613548314624%Z.
+Lemma pmod: p mod 4 =? 3 = true.
+Proof. apply Z.eqb_eq; auto. Qed.
 
-Eval compute in ((( 7 * mp)) mod 2 ^ 64) - 2^64.
+Lemma p_prime: (prime p).
+Proof. Admitted.
+ (* assert (p = Mp 127) as Hmp by reflexivity; rewrite Hmp; 
+    exact (LucasTest 127 (refl_equal _)). 
+Qed. *)
 
-Definition mmod := WordByWordMontgomery.mulmod 64 1 7 mp.
+Notation "x +Fp y" := (GZnZ.add p x y) (at level 100).
+Notation "x *Fp y" := (GZnZ.mul p x y) (at level 90).
+Notation "x -Fp y" := (GZnZ.sub p x y) (at level 100).
 
-Check mmod.
+(*Base field arithmetic, encoding and decoding*)
+Definition mulp x y := (WordByWordMontgomery.mulmod 64 2 p 1 x y).
+Definition addp x y := (WordByWordMontgomery.addmod 64 2 p x y).
+Definition subp x y := (WordByWordMontgomery.submod 64 2 p x y).
+Definition tomont z := WordByWordMontgomery.encodemod 64 2 p 1 z.
+Definition evalp z := @WordByWordMontgomery.eval 64 2 (WordByWordMontgomery.from_montgomerymod 64 2 p 1 z).
 
-Definition reifiablemul127 x1 x2 y1 y2 := (let prod := mul127 [x1; x2] [y1; y2] in (hd prod, hd (tl prod))). 
-
-Definition testfun (x y : Z) := ((mmod [x] [y]), x).
-
-Check testfun.
+Local Notation "x '+p' y" := (addp x y) (at level 100).
+Local Notation "x *p y" := (mulp x y) (at level 90).
+Local Notation "x -p y" := (subp x y) (at level 100).
 
 
-*)
-
-Local Existing Instance ToString.C.OutputCAPI.
-Local Instance : static_opt := true.
-Local Instance : internal_static_opt := true.
-Local Instance : emit_primitives_opt := true.
-(*
-Eval compute in ((-7905747460161236992) mod 2^64).
-
-Definition mp := 10540996613548314624%Z.
-
-Time Redirect "log" Compute
-  (Pipeline.BoundsPipelineToString
-     "fiat_" "fiat_mul127_u64"
-        true None [1] 64
-        ltac:(let r := Reify (testfun) in
-              exact r)
-               (fun _ _ => [])
-               (Some r[0~>2^64-1], (Some r[0~>2^64-1], tt))%zrange
-               (None, Some r[0~>2^64 - 1])%zrange).
-
-
-*)
-Local Notation "x '+p' y" := (add127 x y) (at level 100).
-Local Notation "x *p y" := (mul127 x y) (at level 90).
-Local Notation "x -p y" := (sub127 x y) (at level 100).
-
-Require Import Crypto.Util.LetIn.
-
+(*Extended field arithmetic encoding and decoding*)
 Definition addFp2 := fun x y => ((fst x) +p (fst y), (snd x) +p (snd y)).
 Definition mulFp2 := fun x y => let '(x1, x2) := x in
     let '(y1, y2) := y in
@@ -166,7 +81,117 @@ Definition mulFp2 := fun x y => let '(x1, x2) := x in
                 v0 -p v1,
                 ((((x1) +p (x2)) *p ((y1) +p (y2))) -p v0) -p v1
             ).
+Definition subFp2 := fun x y => ((fst x) -p (fst y), (snd x) -p (snd y)). 
 
+Definition tomontFp2:= fun x => (tomont (val p (fst x)), tomont (val p (snd x))).
+Definition evalFp2:= fun x => (evalp (fst x) zmod p, evalp (snd x) zmod p).
+
+
+(*A few auxillary results on field arithmetic*)
+Add Field fp : (FZpZ p p_prime).
+Lemma Fp2_opp_sub_equiv: forall x y z w, (x *Fp y +Fp ((-1 zmod p) *Fp z) *Fp w) = (x *Fp y -Fp (z *Fp w)).
+Proof. intros. assert (H: (-1 zmod p) = GZnZ.opp p (one p)) by auto; rewrite H; ring. Qed.
+
+Lemma zpz_le_p: forall x, 0 <= val p x < p.
+Proof.
+    intros x; case x; intros val Hval; simpl; rewrite Hval; apply Z_mod_lt; unfold p; auto with zarith.
+Qed.
+
+Lemma karatsuba_correct: forall x1 x2 y1 y2, ((x1 +Fp x2) *Fp (y1 +Fp y2) -Fp x1 *Fp y1 -Fp x2 *Fp y2) = (x1 *Fp y2 +Fp x2 *Fp y1).
+Proof. intros; ring. Qed.
+
+
+(*Proofs of validity (as in Crypto.Arithmetic.WordByWordMontgomery)*)
+Lemma tomont_valid: forall x, WordByWordMontgomery.valid 64 2 p (tomont (val p x)).
+Proof.
+    intros; unfold tomont; pose proof WordByWordMontgomery.encodemod_correct 64 2 p (2^63) 1. destruct H as [_ H0];
+    [auto| auto| lia| unfold p; lia| auto| unfold p; lia|]; apply H0; case x; intros; auto; simpl; rewrite inZnZ; apply Z_mod_lt; unfold p; lia.
+Qed.
+
+Lemma add_valid: forall x y,WordByWordMontgomery.valid 64 2 p x -> WordByWordMontgomery.valid 64 2 p y -> WordByWordMontgomery.valid 64 2 p (x +p y).
+Proof.
+    intros x y Hx Hy; pose proof WordByWordMontgomery.addmod_correct 64 2 p (2^63) 1; destruct H as [_ H0];
+    [auto| auto| lia| unfold p; lia| auto| unfold p; lia|]; apply H0; auto.
+Qed.
+
+Lemma sub_valid: forall x y,WordByWordMontgomery.valid 64 2 p x -> WordByWordMontgomery.valid 64 2 p y -> WordByWordMontgomery.valid 64 2 p (x -p y).
+Proof.
+    intros x y Hx Hy; pose proof WordByWordMontgomery.submod_correct 64 2 p (2^63) 1; destruct H as [_ H0];
+    [auto| auto| lia| unfold p; lia| auto| unfold p; lia|]; apply H0; auto.
+Qed.
+
+Lemma mul_valid: forall x y,WordByWordMontgomery.valid 64 2 p x -> WordByWordMontgomery.valid 64 2 p y -> WordByWordMontgomery.valid 64 2 p (x *p y).
+Proof.
+    intros x y Hx Hy. pose proof WordByWordMontgomery.mulmod_correct 64 2 p (2^63) 1. destruct H;
+    [auto| auto| lia| unfold p; lia| auto| unfold p; lia|]. apply H0; auto.
+Qed.
+
+
+(*Correctness of evaluation wrt. operations and encoding*)
+Theorem eval_tomont_inv: forall val, 0 <= val < p -> evalp (tomont val) mod p = val.
+Proof.
+    intros val H; unfold evalp, tomont; rewrite WordByWordMontgomery.eval_encodemod with (r' := 2 ^ 63);
+    (unfold p, s, c; simpl; unfold Z.pow_pos; simpl; auto with zarith; lia).
+Qed.
+
+Lemma eval_sub: forall x y, WordByWordMontgomery.valid 64 2 p x -> WordByWordMontgomery.valid 64 2 p y -> (evalp (x -p y)) mod p = ( evalp x - evalp y ) mod p.
+Proof. intros; unfold evalp; rewrite WordByWordMontgomery.eval_submod with (r' := 2 ^ 63); auto; try (unfold p; lia). Qed.
+
+Lemma eval_add: forall x y, WordByWordMontgomery.valid 64 2 p x -> WordByWordMontgomery.valid 64 2 p y -> (evalp (x +p y)) mod p = ( evalp x + evalp y ) mod p.
+Proof. intros; unfold evalp; rewrite WordByWordMontgomery.eval_addmod with (r' := 2 ^ 63); auto; try (unfold p; lia). Qed.
+
+Lemma eval_mul: forall x y, WordByWordMontgomery.valid 64 2 p x -> WordByWordMontgomery.valid 64 2 p y -> (evalp (x *p y)) mod p = ( evalp x * evalp y ) mod p.
+Proof. intros; unfold evalp; rewrite WordByWordMontgomery.eval_mulmod with (r' := 2 ^ 63); auto; try (unfold p; lia). Qed.
+
+Lemma eval_sub_mod: forall x y, WordByWordMontgomery.valid 64 2 p x -> WordByWordMontgomery.valid 64 2 p y -> (evalp (x -p y)) mod p = ( evalp x mod p - evalp y mod p ) mod p.
+Proof. intros; rewrite eval_sub; try assumption; apply Zminus_mod. Qed.
+
+Lemma eval_add_mod: forall x y, WordByWordMontgomery.valid 64 2 p x -> WordByWordMontgomery.valid 64 2 p y -> (evalp (x +p y)) mod p = ( evalp x mod p + evalp y mod p ) mod p.
+Proof. intros; rewrite eval_add; try assumption; apply Z.add_mod; unfold p; auto with zarith. Qed.
+
+Lemma eval_mul_mod: forall x y, WordByWordMontgomery.valid 64 2 p x -> WordByWordMontgomery.valid 64 2 p y -> (evalp (x *p y)) mod p = ( evalp x mod p * (evalp y mod p) ) mod p.
+Proof. intros; rewrite eval_mul; try assumption; apply Z.mul_mod; unfold p; auto with zarith. Qed.
+
+
+(*Correctness of extended field operations and encoding*)
+Theorem addFp2_correct: forall x y, evalFp2 (addFp2 (tomontFp2 x) (tomontFp2 y)) = addp2 p x y.
+Proof.
+    intros; apply Fp2irr; simpl; apply zirr; rewrite eval_add_mod; try apply tomont_valid;
+    repeat rewrite eval_tomont_inv; auto; apply zpz_le_p.
+Qed.
+
+Theorem subFp2_correct: forall x y , evalFp2 (subFp2 (tomontFp2 x) (tomontFp2 y)) = subp2 p x y.
+Proof.
+    intros; apply Fp2irr; simpl; apply zirr; rewrite eval_sub_mod; try apply tomont_valid;
+    repeat rewrite eval_tomont_inv; auto; apply zpz_le_p.
+Qed.
+
+Theorem mul_correct: forall x y, evalFp2 (mulFp2 (tomontFp2 x) (tomontFp2 y)) = mulp2 p x y.
+Proof.
+    intros x y. unfold mulFp2, mulp2. rewrite quad_res_minus_1. simpl. apply Fp2irr.
+    - simpl; rewrite Fp2_opp_sub_equiv; apply zirr; rewrite eval_sub_mod; try (apply mul_valid; apply tomont_valid);
+      repeat rewrite eval_mul_mod; try apply tomont_valid; repeat rewrite eval_tomont_inv; try apply zpz_le_p; reflexivity.
+    - rewrite <- karatsuba_correct; simpl; apply zirr; repeat rewrite eval_sub_mod;
+      [| apply mul_valid; apply add_valid; apply tomont_valid
+       | apply mul_valid; apply tomont_valid
+       | apply sub_valid; apply mul_valid; [apply add_valid| apply add_valid| |]; apply tomont_valid
+       | apply mul_valid; apply tomont_valid].
+      rewrite eval_mul_mod; try ( try apply add_valid; apply tomont_valid);
+      repeat rewrite eval_mul_mod; try apply tomont_valid;
+      rewrite eval_add_mod; try apply tomont_valid;
+      rewrite eval_add_mod; try apply tomont_valid; repeat rewrite eval_tomont_inv; try apply zpz_le_p; reflexivity.
+Qed.
+
+Theorem to_montFp2_correct: forall x y, evalFp2 (tomontFp2 (x, y)) = (x, y).
+Proof.
+    intros x y; apply injective_projections; [case x | case y];
+    intros val Hval; apply zirr; simpl; apply eval_tomont_inv;
+    rewrite Hval; apply Z_mod_lt; unfold p, c, s; simpl; lia.
+Qed.
+
+(*Reification and subsequent printing to C of field operations.
+  Note that a slightly altered implementation of operations are used;
+  their equivalence is shown below. *)
 Definition  mulFp2r x1 x2 y1 y2 :=
         dlet v0 := (x1) *p (y1) in 
         dlet v1 := (x2) *p (y2) in
@@ -179,361 +204,101 @@ Definition  mulFp2r x1 x2 y1 y2 :=
                                 v3 -p v1
             ).
 
+Lemma mulFp2r_correct: forall x y, mulFp2r (fst x) (snd x) (fst y) (snd y) = mulFp2 x y.
+Proof. intros x y; destruct x, y. auto. Qed.
 
-Definition mulFp2reif (x11 x12 x21 x22 y11 y12 y21 y22 : Z) := let '(z1, z2) := (mulFp2 ([x11; x12], [x21; x22]) ([y11; y12], [y21; y22])) in
-    [nth_default 0 z1 0; nth_default 1 z1 0; nth_default 0 z2 0; nth_default 1 z2 0].
-(*
-Definition mulFp2r (x1 x2 y1 y2 : list Z) := mulFp2 (x1, x2) (y1, y2).
-*)
-Definition hej (l1 l2 l3 l4: list Z) : list Z :=
-    l1 +p l2 +p l3.
+Definition addFp2r x1 x2 y1 y2 := (x1 +p y1, x2 +p y2).
 
-Definition hej2 x1 x2 y1 y2 :=
-    (dlet v0 := (x1 +p y1) in (
-            dlet v1 := (x2 +p y2) in (
-                x1,
-                x2
-            )
-        )
-    ).
+Lemma addFp2r_correct: forall x y, addFp2r (fst x) (snd x) (fst y) (snd y) = addFp2 x y.
+Proof. intros x y; destruct x, y; auto. Qed.
 
-Definition to_montgomeryFp2 x := (tomont127 (val p (fst x)), tomont127 (val p (snd x))).
+Definition subFp2r x1 x2 y1 y2 := (x1 -p y1, x2 -p y2).
 
+Lemma subFp2r_correct: forall x y, subFp2r (fst x) (snd x) (fst y) (snd y) = subFp2 x y.
+Proof. intros x y; destruct x, y; auto. Qed.
 
-Definition eval_Fp2 x :=
-    (
-        eval127(fst x) zmod p,
-        eval127(snd x) zmod p
-    ).
+(*Initializing parameters for reification*)
+Local Instance : split_mul_to_opt := None.
+Local Instance : split_multiret_to_opt := None.
+Local Instance : unfold_value_barrier_opt := true.
+Local Instance : only_signed_opt := false.
+Local Instance : no_select_size_opt := None.
+Local Existing Instance default_low_level_rewriter_method.
+Local Existing Instance ToString.C.OutputCAPI.
+Local Instance : static_opt := true.
+Local Instance : internal_static_opt := true.
+Local Instance : emit_primitives_opt := true.
 
-(*
-Time Redirect "log" Compute
+Compute
      (Pipeline.BoundsPipelineToString
-        "fiat_" "fial_mulFp2_"
-        false None [64; 128] 64
+        "fiat_" "fiat_mulFp2_"
+        false None [1; 64; 128] 64
         ltac:(let r := Reify (mulFp2r) in
               exact r)
               (fun _ _ => [])
               (Some (repeat (Some r[0~>2^64 - 1]) 2), (Some (repeat (Some r[0~>2^64 - 1]) 2), (Some (repeat (Some r[0~>2^64 - 1]) 2) , (Some (repeat (Some r[0~>2^64 - 1]) 2), tt))))%zrange
               (Some (repeat (Some r[0~>2^64 - 1]) 2), Some (repeat (Some r[0~>2^64 - 1]) 2))%zrange).
-*)
 
-Lemma eval_correct: forall x, x = ((eval127 (tomont127 (val p x))) zmod p).
-Proof.
-    intros x. case x. simpl. intros val inZnZ. apply zirr. unfold eval127, tomont127. Check WordByWordMontgomery.eval_encodemod.
-    rewrite WordByWordMontgomery.eval_encodemod with (r' := 2 ^63); try auto; unfold p, c, s; simpl; unfold Z.pow_pos; simpl; try lia.
-    rewrite inZnZ. unfold p, c, s; simpl. apply Z_mod_lt. lia.
-Qed.
+Compute
+     (Pipeline.BoundsPipelineToString
+     "fiat_" "fiat_addFp2_"
+     false None [1; 64; 128] 64
+     ltac:(let r := Reify (addFp2r) in
+           exact r)
+           (fun _ _ => [])
+           (Some (repeat (Some r[0~>2^64 - 1]) 2), (Some (repeat (Some r[0~>2^64 - 1]) 2), (Some (repeat (Some r[0~>2^64 - 1]) 2) , (Some (repeat (Some r[0~>2^64 - 1]) 2), tt))))%zrange
+           (Some (repeat (Some r[0~>2^64 - 1]) 2), Some (repeat (Some r[0~>2^64 - 1]) 2))%zrange).
 
+Compute
+     (Pipeline.BoundsPipelineToString
+     "fiat_" "fiat_subFp2_"
+     false None [1; 64; 128] 64
+     ltac:(let r := Reify (subFp2r) in
+           exact r)
+           (fun _ _ => [])
+           (Some (repeat (Some r[0~>2^64 - 1]) 2), (Some (repeat (Some r[0~>2^64 - 1]) 2), (Some (repeat (Some r[0~>2^64 - 1]) 2) , (Some (repeat (Some r[0~>2^64 - 1]) 2), tt))))%zrange
+           (Some (repeat (Some r[0~>2^64 - 1]) 2), Some (repeat (Some r[0~>2^64 - 1]) 2))%zrange).
 
-Lemma eval_compat: forall x n, Positional.eval w n x = @WordByWordMontgomery.eval 64 n x.
-Proof. auto. Qed.
+(* The generated code makes calls to the functions; fiat_cmovznz_u64,
+   fiat_addcarryx_u64, fiat_subborrowx_u64 and fiat_mulx_u64.
+   These can be generated with the following.*)
 
-Lemma eval_encode: forall x n, n <> 0%nat -> Positional.eval w n (Positional.encode w n s c x) mod p = x mod p.
-Proof.
-    intros. apply Positional.eval_encode; (unfold s, c, p; auto with zarith; try lia).
-    - intros. unfold w, uweight. assert (0 < weight 64 1 i). apply weight_positive, wprops; lia. lia.
-    - simpl; lia.
-    - intros. unfold w, uweight. assert (0 < (weight 64 1 (S i)) / (weight 64 1 i)). apply weight_divides, wprops; lia. lia.
-Qed.
+Compute
+  (Pipeline.BoundsPipelineToString
+     "fiat_" "fiat_cmovznz_u64"
+        true None [1; 64; 128] 64
+        ltac:(let r := Reify (cmovznz 64) in
+              exact r)
+               (fun _ _ => [])
+               (Some r[0~>1], (Some r[0~>2^64-1], (Some r[0~>2^64-1], tt)))%zrange
+               (Some r[0~>2^64-1])%zrange).
 
+Compute
+    (Pipeline.BoundsPipelineToString
+        "fiat_" "fiat_subborrowx_u64"
+            true None [1; 64; 128] 64
+            ltac:(let r := Reify (subborrowx 64) in
+             exact r)
+                (fun _ _ => [])
+                (Some r[0~>1], (Some r[0~>2^64-1], (Some r[0~>2^64-1], tt)))%zrange
+                (Some r[0~>2^64-1], Some r[0~>1])%zrange).
 
-Eval compute in (uweight 64 1).
+Compute
+(Pipeline.BoundsPipelineToString
+   "fiat_" "fiat_addcarryx_u64"
+      true None [1; 64; 128] 64
+      ltac:(let r := Reify (addcarryx 64) in
+            exact r)
+             (fun _ _ => [])
+             (Some r[0~>1], (Some r[0~>2^64-1], (Some r[0~>2^64-1], tt)))%zrange
+             (Some r[0~>2^64-1], Some r[0~>1])%zrange).
 
-Theorem eval_tomont_inv: forall val, 0 <= val < p -> eval127 (tomont127 val) mod p = val.
-Proof.
-    intros val H; unfold eval127, tomont127; rewrite WordByWordMontgomery.eval_encodemod with (r' := 2 ^ 63);
-    (unfold p, s, c; simpl; unfold Z.pow_pos; simpl; auto with zarith; lia).
-Qed.
-
-
-Theorem to_montFp2_correct: forall x y, eval_Fp2 (to_montgomeryFp2 (x, y)) = (x, y).
-Proof.
-    intros; unfold eval_Fp2; apply injective_projections; [case x | case y];
-    intros val Hval; apply zirr; simpl; apply eval_tomont_inv;
-    rewrite Hval; apply Z_mod_lt; unfold p, c, s; simpl; lia.
-Qed.
-
-Definition tomontFp2:= fun x => (tomont127 (val p (fst x)), tomont127 (val p (snd x))).
-Definition evalFp2:= fun x => (eval127 (fst x) zmod p, eval127 (snd x) zmod p).
-
-Local Ltac thisauto := unfold p, c, s; simpl; unfold Z.pow_pos; simpl; auto with zarith.
-
-
-(*SKRIV DETTE RENT!!!!!*)
-Theorem add127_correct: forall x y, (eval127(tomont127 (val p x) +p tomont127 (val p y)) zmod p) = (x +Fp y).
-Proof.
-    intros x y. unfold add127. unfold add. simpl. apply zirr. unfold eval127.
-    rewrite WordByWordMontgomery.eval_addmod with (r' := 2 ^ 63); [|thisauto|thisauto|thisauto|thisauto|thisauto|thisauto| | ].
-        - unfold tomont127. rewrite PullPush.Z.add_mod_full.
-        assert  (forall z, (@WordByWordMontgomery.eval 64 2
-                (WordByWordMontgomery.from_montgomerymod 64 2 p 1
-                (WordByWordMontgomery.encodemod 64 2 p 1 z)) mod p)
-           = eval127 (tomont127 z) mod p); [auto|].
-        do 2 rewrite H.
-        repeat rewrite eval_tomont_inv; try reflexivity;
-        [destruct y| destruct x]; simpl; rewrite inZnZ; apply Z_mod_lt; thisauto.
-        - pose proof WordByWordMontgomery.encodemod_correct 64 2 p (2 ^ 63) 1. apply H;
-          try ( unfold p, c, s; simpl; unfold Z.pow_pos; simpl; auto with zarith; lia).
-          destruct x. simpl. rewrite inZnZ. apply Z_mod_lt. unfold p, c, s; simpl; lia.
-        - unfold tomont127.
-          pose proof WordByWordMontgomery.encodemod_correct 64 2 p (2 ^ 63) 1. apply H;
-          try ( unfold p, c, s; simpl; unfold Z.pow_pos; simpl; auto with zarith; lia).
-          destruct y. simpl. rewrite inZnZ. apply Z_mod_lt. unfold p, c, s; simpl; lia.
-Qed.
-
-Theorem add127_corr: forall x y, (eval127((tomont127 (val p x)) +p (tomont127 (val p y))) zmod p) = (eval127 (tomont127 (val p (x +Fp y))) zmod p).
-Proof.
-    intros x y. rewrite add127_correct. apply zirr. rewrite eval_tomont_inv; auto.
-    case x, y. simpl. apply Z.mod_pos_bound. unfold p. lia.
-Qed. 
-
-Theorem add_correct: forall x y, evalFp2 (addFp2 (tomontFp2 x) (tomontFp2 y)) = addp2 p x y.
-Proof.
-    intros x y. unfold evalFp2, tomontFp2. simpl. unfold addp2. apply injective_projections; (simpl; rewrite add127_correct; reflexivity).
-Qed.
-
-
-Theorem mul127_correct: forall x y, (eval127 (tomont127 (val p x) *p tomont127 (val p y)) zmod p) = (x *Fp y).
-Proof.
-    intros x y. unfold mul127. unfold mul. simpl. apply zirr. unfold eval127.
-    rewrite WordByWordMontgomery.eval_mulmod with (r' := 2 ^ 63); [|thisauto|thisauto|thisauto|thisauto|thisauto|thisauto| | ].
-        - unfold tomont127. rewrite Z.mul_mod; [| unfold p, c, s; simpl; auto with zarith].
-        assert  (forall z, (@WordByWordMontgomery.eval 64 2
-                (WordByWordMontgomery.from_montgomerymod 64 2 p 1
-                (WordByWordMontgomery.encodemod 64 2 p 1 z)) mod p)
-           = eval127 (tomont127 z) mod p); [auto|].
-        do 2 rewrite H.
-        repeat rewrite eval_tomont_inv; try reflexivity;
-        [destruct y| destruct x]; simpl; rewrite inZnZ; apply Z_mod_lt; thisauto.
-        - pose proof WordByWordMontgomery.encodemod_correct 64 2 p (2 ^ 63) 1. apply H;
-          try ( unfold p, c, s; simpl; unfold Z.pow_pos; simpl; auto with zarith; lia).
-          destruct x. simpl. rewrite inZnZ. apply Z_mod_lt. unfold p, c, s; simpl; lia.
-        - unfold tomont127.
-          pose proof WordByWordMontgomery.encodemod_correct 64 2 p (2 ^ 63) 1. apply H;
-          try ( unfold p, c, s; simpl; unfold Z.pow_pos; simpl; auto with zarith; lia).
-          destruct y. simpl. rewrite inZnZ. apply Z_mod_lt. unfold p, c, s; simpl; lia.
-Qed.
-
-Theorem mul127_corr: forall x y, (eval127((tomont127 (val p x)) *p (tomont127 (val p y))) zmod p) = (eval127 (tomont127 (val p (x *Fp y))) zmod p).
-Proof.
-    intros x y. rewrite mul127_correct. apply zirr. rewrite eval_tomont_inv; auto.
-    case x, y. simpl. apply Z.mod_pos_bound. unfold p. lia.
-Qed.
-
-Theorem sub127_correct: forall x y, (eval127 (tomont127 (val p x) -p tomont127 (val p y)) zmod p) = (x -Fp y).
-Proof.
-    intros x y. unfold sub127. unfold sub. simpl. apply zirr. unfold eval127.
-    rewrite WordByWordMontgomery.eval_submod with (r' := 2 ^ 63); [|thisauto|thisauto|thisauto|thisauto|thisauto|thisauto| | ].
-        - unfold tomont127. rewrite Zminus_mod.
-        assert  (forall z, (@WordByWordMontgomery.eval 64 2
-                (WordByWordMontgomery.from_montgomerymod 64 2 p 1
-                (WordByWordMontgomery.encodemod 64 2 p 1 z)) mod p)
-           = eval127 (tomont127 z) mod p); [auto|].
-        do 2 rewrite H.
-        repeat rewrite eval_tomont_inv; try reflexivity;
-        [destruct y| destruct x]; simpl; rewrite inZnZ; apply Z_mod_lt; thisauto.
-        - pose proof WordByWordMontgomery.encodemod_correct 64 2 p (2 ^ 63) 1. apply H;
-          try ( unfold p, c, s; simpl; unfold Z.pow_pos; simpl; auto with zarith; lia).
-          destruct x. simpl. rewrite inZnZ. apply Z_mod_lt. unfold p, c, s; simpl; lia.
-        - unfold tomont127.
-          pose proof WordByWordMontgomery.encodemod_correct 64 2 p (2 ^ 63) 1. apply H;
-          try ( unfold p, c, s; simpl; unfold Z.pow_pos; simpl; auto with zarith; lia).
-          destruct y. simpl. rewrite inZnZ. apply Z_mod_lt. unfold p, c, s; simpl; lia.
-Qed.
-
-Theorem sub127_corr: forall x y, (eval127((tomont127 (val p x)) -p (tomont127 (val p y))) zmod p) = (eval127 (tomont127 (val p (x -Fp y))) zmod p).
-Proof.
-    intros x y. rewrite sub127_correct. apply zirr. rewrite eval_tomont_inv; auto.
-    case x, y. simpl. apply Z.mod_pos_bound. unfold p. lia.
-Qed.
-
-Theorem sub127_corr2: forall x y, (tomont127 (val p x) -p (tomont127 (val p y))) = tomont127 (val p (x -Fp y)).
-Proof.
-    intros x y. unfold sub127. Abort.
-
-
-
-Add Field fp : (FZpZ p p_prime).
-
-Lemma Fp2irr': forall x, val p (x zmod p) = x mod p.
-Proof. auto. Qed.
-
-Lemma Fp2aux: forall x, val p x = val p x mod p.
-Proof. intros. case x. intros. simpl. auto. Qed.
-
-Lemma auxFp: forall x, -x  = (-1) * x.
-Proof. auto. Qed.
-
-Lemma Fp2_l1: forall x, ((-1 zmod p) *Fp x) = GZnZ.opp p x.
-Proof.
-    intros. apply zirr. auto with zarith. rewrite  Fp2irr'. rewrite Fp2aux. rewrite <- Z.mul_mod.
-        - rewrite (auxFp (val p x mod p)). rewrite Z.mul_mod with (b := (val p x mod p)); try (unfold p; lia). rewrite Z.mod_mod; try (unfold p; lia). auto with zarith.
-        - unfold p; lia.
-Qed.
-
-Lemma Fp2_l2: forall x y, ((GZnZ.opp p x) *Fp y) = GZnZ.opp p (x *Fp y).
-Proof. intros; ring. Qed.
-
-Lemma Fp2_l3: forall x y, (x +Fp (GZnZ.opp p y)) = (x -Fp y).
-Proof. intros; ring. Qed.
-
-Lemma Fp2aux2: forall x y z w, (x *Fp y +Fp ((-1 zmod p) *Fp z) *Fp w) = (x *Fp y -Fp (z *Fp w)).
-Proof.
-    intros. rewrite Fp2_l1, Fp2_l2, Fp2_l3. auto.
-Qed.
-
-Lemma tomont_valid: forall x, WordByWordMontgomery.valid 64 2 p (tomont127 (val p x)).
-Proof.
-    intros. unfold tomont127. pose proof WordByWordMontgomery.encodemod_correct 64 2 p (2^63) 1. destruct H;
-    [auto| auto| lia| unfold p; lia| auto| unfold p; lia|]. apply H0. case x. intros; auto. simpl. rewrite inZnZ. apply Z_mod_lt. unfold p. lia.
-Qed.
-
-Lemma add_valid: forall x y,WordByWordMontgomery.valid 64 2 p x -> WordByWordMontgomery.valid 64 2 p y -> WordByWordMontgomery.valid 64 2 p (x +p y).
-Proof.
-    intros x y Hx Hy. pose proof WordByWordMontgomery.addmod_correct 64 2 p (2^63) 1. destruct H;
-    [auto| auto| lia| unfold p; lia| auto| unfold p; lia|]. apply H0; auto.
-Qed.
-
-Lemma sub_valid: forall x y,WordByWordMontgomery.valid 64 2 p x -> WordByWordMontgomery.valid 64 2 p y -> WordByWordMontgomery.valid 64 2 p (x -p y).
-Proof.
-    intros x y Hx Hy; pose proof WordByWordMontgomery.submod_correct 64 2 p (2^63) 1; destruct H as [_ H0];
-    [auto| auto| lia| unfold p; lia| auto| unfold p; lia|]; apply H0; auto.
-Qed.
-
-Lemma add_valid_corr: forall x y, WordByWordMontgomery.valid 64 2 p (tomont127 (val p x) +p tomont127 (val p y)).
-Proof.
-    intros x y; apply add_valid; apply tomont_valid.
-Qed.
-
-Lemma mul_valid: forall x y,WordByWordMontgomery.valid 64 2 p x -> WordByWordMontgomery.valid 64 2 p y -> WordByWordMontgomery.valid 64 2 p (x *p y).
-Proof.
-    intros x y Hx Hy. pose proof WordByWordMontgomery.mulmod_correct 64 2 p (2^63) 1. destruct H;
-    [auto| auto| lia| unfold p; lia| auto| unfold p; lia|]. apply H0; auto.
-Qed.
-
-Lemma mul_valid_corr: forall x y, WordByWordMontgomery.valid 64 2 p (tomont127 (val p x) *p tomont127 (val p y)).
-Proof.
-    intros x y; apply mul_valid; apply tomont_valid.
-Qed.
-
-Lemma zpz_le_p: forall x, 0 <= val p x < p.
-Proof.
-    intros x. case x. intros val Hval. simpl. rewrite Hval. apply Z_mod_lt. unfold p; auto with zarith.
-Qed.
-
-Lemma karatsuba_correct: forall x1 x2 y1 y2, ((x1 +Fp x2) *Fp (y1 +Fp y2) -Fp x1 *Fp y1 -Fp x2 *Fp y2) = (x1 *Fp y2 +Fp x2 *Fp y1).
-Proof. intros; ring. Qed.
-
-Lemma eval_sub: forall x y, WordByWordMontgomery.valid 64 2 p x -> WordByWordMontgomery.valid 64 2 p y -> (eval127 (x -p y)) mod p = ( eval127 x - eval127 y ) mod p.
-Proof. intros; unfold eval127; rewrite WordByWordMontgomery.eval_submod with (r' := 2 ^ 63); auto; try (unfold p; lia). Qed.
-
-Lemma eval_add: forall x y, WordByWordMontgomery.valid 64 2 p x -> WordByWordMontgomery.valid 64 2 p y -> (eval127 (x +p y)) mod p = ( eval127 x + eval127 y ) mod p.
-Proof. intros; unfold eval127; rewrite WordByWordMontgomery.eval_addmod with (r' := 2 ^ 63); auto; try (unfold p; lia). Qed.
-
-Lemma eval_mul: forall x y, WordByWordMontgomery.valid 64 2 p x -> WordByWordMontgomery.valid 64 2 p y -> (eval127 (x *p y)) mod p = ( eval127 x * eval127 y ) mod p.
-Proof. intros; unfold eval127; rewrite WordByWordMontgomery.eval_mulmod with (r' := 2 ^ 63); auto; try (unfold p; lia). Qed.
-
-Lemma eval_sub_mod: forall x y, WordByWordMontgomery.valid 64 2 p x -> WordByWordMontgomery.valid 64 2 p y -> (eval127 (x -p y)) mod p = ( eval127 x mod p - eval127 y mod p ) mod p.
-Proof. intros; rewrite eval_sub; try assumption; apply Zminus_mod. Qed.
-
-Lemma eval_add_mod: forall x y, WordByWordMontgomery.valid 64 2 p x -> WordByWordMontgomery.valid 64 2 p y -> (eval127 (x +p y)) mod p = ( eval127 x mod p + eval127 y mod p ) mod p.
-Proof. intros; rewrite eval_add; try assumption; apply Z.add_mod; unfold p; auto with zarith. Qed.
-
-Lemma eval_mul_mod: forall x y, WordByWordMontgomery.valid 64 2 p x -> WordByWordMontgomery.valid 64 2 p y -> (eval127 (x *p y)) mod p = ( eval127 x mod p * (eval127 y mod p) ) mod p.
-Proof. intros; rewrite eval_mul; try assumption; apply Z.mul_mod; unfold p; auto with zarith. Qed.
-
-
-Theorem mul_correct: forall x y, evalFp2 (mulFp2 (tomontFp2 x) (tomontFp2 y)) = mulp2 p x y.
-Proof.
-    intros x y. unfold mulFp2, mulp2. rewrite quad_res_minus_1. simpl. apply Fp2irr.
-    - simpl. rewrite Fp2aux2. apply zirr. rewrite eval_sub_mod; try (apply mul_valid; apply tomont_valid).
-      repeat rewrite eval_mul_mod; try apply tomont_valid. repeat rewrite eval_tomont_inv; try apply zpz_le_p. reflexivity.
-    - rewrite <- karatsuba_correct. simpl. apply zirr. repeat rewrite eval_sub_mod;
-      [| apply mul_valid; apply add_valid; apply tomont_valid
-       | apply mul_valid; apply tomont_valid
-       | apply sub_valid; apply mul_valid; [apply add_valid| apply add_valid| |]; apply tomont_valid
-       | apply mul_valid; apply tomont_valid].
-      rewrite eval_mul_mod; try ( try apply add_valid; apply tomont_valid).
-      repeat rewrite eval_mul_mod; try apply tomont_valid.
-      rewrite eval_add_mod; try apply tomont_valid. unfold GZnZ.add, GZnZ.mul, GZnZ.sub. 
-    
-    
-    
-    unfold eval127. rewrite WordByWordMontgomery.eval_submod with (r' := 2^63);
-    [|auto with zarith| auto with zarith | lia | unfold p; lia | auto | unfold p; lia | | apply mul_valid_corr].
-        + rewrite Zminus_mod.
-          repeat rewrite WordByWordMontgomery.eval_mulmod with (r' := 2^63);
-          [|auto with zarith | auto with zarith | lia | unfold p; lia | auto | unfold p; lia| apply tomont_valid| apply tomont_valid ].
-          rewrite Z.mul_mod; [| unfold p; auto with zarith]. 
-          assert  (H :forall z, (@WordByWordMontgomery.eval 64 2
-          (WordByWordMontgomery.from_montgomerymod 64 2 p 1
-          (WordByWordMontgomery.encodemod 64 2 p 1 z)) mod p)
-            = eval127 (tomont127 z) mod p); [auto|].
-          rewrite H. rewrite H. unfold GZnZ.mul. remember (val p (fst x)) as x1. remember (val p (snd x)) as x2. remember (val p (fst y)) as y1.
-          remember (val p (snd y)) as y2. remember (tomont127 x1) as vx1. remember (tomont127 x2) as vx2. remember (tomont127 y1) as vy1. remember (tomont127 y2) as vy2.
-          rewrite <- Z.mul_mod. subst vx1. unfold sub127. rewrite WordByWordMontgomery.eval_submod with (r' := 2 ^ 63);
-          [|auto with zarith | auto with zarith | lia | unfold p; lia | auto | unfold p; lia | | ].
-           rewrite Zminus_mod  with (b := WordByWordMontgomery.eval 64
-           (WordByWordMontgomery.from_montgomerymod 64 2 p 1 (tomont127 x1 *p vy1))).
-           rewrite WordByWordMontgomery.eval_mulmod with (r' := 2^63);
-           [|auto with zarith | auto with zarith | lia | unfold p; lia | auto | unfold p; lia | | ].
-           rewrite Z.mul_mod.
-           rewrite WordByWordMontgomery.eval_addmod with (r' := 2 ^ 63); [|auto with zarith | auto with zarith | lia | unfold p; lia | auto | unfold p; lia | | ].
-           rewrite WordByWordMontgomery.eval_addmod with (r' := 2^63); [|auto with zarith | auto with zarith | lia | unfold p; lia | auto | unfold p; lia | | ].
-           rewrite WordByWordMontgomery.eval_mulmod with (r' := 2 ^ 63); [|auto with zarith | auto with zarith | lia | unfold p; lia | auto | unfold p; lia | | ].
-           subst vx2 vy1 vy2. unfold tomont127. unfold eval127. rewrite Z.add_mod. rewrite H. rewrite H.
-           rewrite Z.add_mod with (b := WordByWordMontgomery.eval 64
-           (WordByWordMontgomery.from_montgomerymod 64 2 p 1
-              (WordByWordMontgomery.encodemod 64 2 p 1 y2))). rewrite H; rewrite H.
-            rewrite Z.mul_mod with (b := WordByWordMontgomery.eval 64
-            (WordByWordMontgomery.from_montgomerymod 64 2 p 1
-               (WordByWordMontgomery.encodemod 64 2 p 1 y1))). rewrite H. rewrite H.
-            rewrite Z.mul_mod with (b := WordByWordMontgomery.eval 64
-            (WordByWordMontgomery.from_montgomerymod 64 2 p 1
-               (WordByWordMontgomery.encodemod 64 2 p 1 y2))). do 2 rewrite H. repeat rewrite eval_tomont_inv. simpl.
-            repeat rewrite <- Z.mul_mod. repeat rewrite <- Zminus_mod. repeat rewrite <- Z.add_mod. subst x1 x2 y1 y2. auto.
-
-            rewrite 
-            
-            auto. rewrite Z.mod_mod. rewrite eval_tomont_inv. rewrite <- Zminus_mod.
-           
-           
-          
-          
-          
-          unfold sub127. rewri rewrite Z.mul_mod with (b := WordByWordMontgomery.eval 64
-          (WordByWordMontgomery.from_montgomerymod 64 2 p 1
-            (WordByWordMontgomery.encodemod 64 2 p 1
-               (val p (snd y))))); [| unfold p; auto with zarith].
-          rewrite H. rewrite H. unfold GZnZ.mul. case x, y. repeat rewrite Crypto.Util.Prod.fst_pair.
-          repeat rewrite Crypto.Util.Prod.snd_pair. repeat rewrite eval_tomont_inv; try apply zpz_le_p;  repeat rewrite Fp2irr'. reflexivity.
-     (*Fortsæt her; skriv tactic til subgoals!!!!!*)
-
-
-     forall x, y: (x + (-1 mod p * y)) mod p = 
-     ring. simpl.
-     
-     simpl. unfold eval127. rewrite WordByWordMontgomery.eval_submod with (r' := 2 ^ 63); try (unfold p; lia; auto).
-        + rewrite Zminus_mod. repeat rewrite WordByWordMontgomery.eval_mulmod with (r' := 2^63); try auto. 
-            * unfold tomont127.
-    simpl. apply zirr. unfold eval127. rewrite WordByWordMontgomery.eval_submod with (r' := 2 ^ 63).
-        - rewrite Zminus_mod. repeat rewrite WordByWordMontgomery.eval_mulmod with (r' := 2^63).
-          repeat rewrite WordByWordMontgomery.eval_mulmod with (r' := 2^63).
-            + unfold tomont127. rewrite Z.mul_mod. rewrite WordByWordMontgomery.eval_encodemod with (r' := 2 ^ 63).
-              rewrite WordByWordMontgomery.eval_encodemod with (r' := 2 ^ 63).
-              pose proof (Z.mul_mod (@WordByWordMontgomery.eval 64 2
-              (WordByWordMontgomery.from_montgomerymod 64
-                 2 p 1
-                 (WordByWordMontgomery.encodemod 64 2 p 1
-                    (val p (snd x))))) ( @WordByWordMontgomery.eval 64 2
-                    (WordByWordMontgomery.from_montgomerymod 64
-                       2 p 1
-                       (WordByWordMontgomery.encodemod 64 2 p 1
-                          (val p (snd y))))) p). rewrite H.
-                          rewrite WordByWordMontgomery.eval_encodemod with (r' := 2 ^ 63).
-              rewrite WordByWordMontgomery.eval_encodemod with (r' := 2 ^ 63).
-              rewrite <- Z.mul_mod. rewrite <- Z.mul_mod. rewrite <- Zminus_mod. rewrite quad_res_minus_1.
-              ring_simplify. unfold mul. assert ((-1 zmod p) = opp p (1 zmod p)). auto. simpl. simpl. ring. 
-    unfold tomont127. rewrite mul_correct. 
-Qed.
+Compute
+(Pipeline.BoundsPipelineToString
+   "fiat_" "fiat_mulx_u64"
+      true None [64; 128] 64
+      ltac:(let r := Reify (mulx 64) in
+            exact r)
+             (fun _ _ => [])
+             (Some r[0~>2^64-1], (Some r[0~>2^64-1], tt))%zrange
+             (Some r[0~>2^64-1], Some r[0~>2^64-1])%zrange).
